\[[<](./p0063.md)] \[[^](../README.md)] | \[[>](./p0065.md)]

# Problem 64: Odd period square roots

## The link to the problem

- [Odd period square roots](https://projecteuler.net/problem=64)

## My approach

Assume that $N$ is not a perfect square, and $\sqrt{N} = \dfrac{\sqrt{N} + b_{0}}{c_{0}} = a_{0} + \dfrac{1}{x_{1}} \ \ (b_{0} = 0, \ c_{0} = 1, \ a_{0} = \lfloor \dfrac{\sqrt{N} + b_{0}}{c_{0}} \rfloor, \ x_{1} > 1)$.

$$
\begin{align}
x_{1} & = \frac{c_{0}}{\sqrt{N} + (b_{0} - a_{0}c_{0})} \\
      & = \frac{c_{0} (\sqrt{N} - (b_{0} - a_{0}c_{0}))}{N - (b_{0} - a_{0}c_{0})^{2}} \\
      & = \frac{\sqrt{N} + (a_{0}c_{0} - b_{0})}{\frac{N - (b_{0} - a_{0}c_{0})^{2}}{c_{0}}}
\end{align}
$$

Let $b_{1} = a_{0} c_{0} - b_{0}, \ c_{1} = \dfrac{N - (b_{0} - a_{0} c_{0})^{2}}{c_{0}}$.

$$
\begin{align}
x_{1} & = \frac{\sqrt{N} + (a_{0}c_{0} - b_{0})}{\frac{N - (b_{0} - a_{0}c_{0})^{2}}{c_{0}}} \\
      & = \frac{\sqrt{N} + b_{1}}{c_{1}}
\end{align}
$$

In a similar way, let $a_{1} = \lfloor \dfrac{\sqrt{N} + b_{1}}{c_{1}} \rfloor, \ x_{2} > 1$. 
$$x_{1} = \frac{\sqrt{N} + b_{1}}{c_{1}} = a_{1} + \frac{1}{x_{2}}$$

Then, if $n \ge 0$:

$$
\begin{align}
a_{n} & = \lfloor \frac{\sqrt{N} + b_{n}}{c_{n}} \rfloor \\
b_{n+1} & = a_{n}c_{n} - b_{n} \\
c_{n+1} & = \frac{N - (b_{n} - a_{n}c_{n})^{2}}{c_{n}} = \frac{N - (a_{n}c_{n} - b_{n})^{2}}{c_{n}} = \frac{N - {b_{n+1}}^{2}}{c_{n}}
\end{align}
$$

Therefore, we can get the period by using above equations.

